height sensitive

ModalLogic/P.lean
@@ -1,4 +1,5 @@
 import ModalLogic.Notations
+import Mathlib.Order.Basic
 import Mathlib.Data.Finset.Basic
 
 namespace Finset
@@ -9,7 +10,7 @@ end Finset
 
 open Nat Finset
 
-attribute [simp] union_self
+attribute [simp] union_self erase_subset
 
 namespace ModalLogic.P
 
@@ -43,6 +44,18 @@ instance : HasBot (Formula α) := ⟨bot⟩
 instance : HasDisj (Formula α) := ⟨disj⟩
 instance : HasConj (Formula α) := ⟨conj⟩
 
+@[simp] lemma conj_neq {φ ψ ξ ζ : Formula α} : (φ ≠ ξ ∨ ψ ≠ ζ) → (φ ⋏ ψ) ≠ (ξ ⋏ ζ) := by
+  intro h;
+  cases h with
+  | inl h => intro h; injection h; contradiction;
+  | inr h => intro h; injection h; contradiction;
+
+@[simp] lemma disj_neq {φ ψ ξ ζ : Formula α} : (φ ≠ ξ ∨ ψ ≠ ζ) → ((φ ⋎ ψ) ≠ (ξ ⋎ ζ)) := by
+  intro h;
+  cases h with
+  | inl h => intro h; injection h; contradiction;
+  | inr h => intro h; injection h; contradiction;
+
 /-
 def isPrime : Formula α → Bool
   | prime _ => true
@@ -60,6 +73,7 @@ instance : HasNeg (Formula α) := ⟨neg⟩
 lemma neg_conj_disj (φ ψ : Formula α) : ~(φ ⋏ ψ) = (~φ) ⋎ (~ψ) := by rfl
 lemma neg_disj_conj (φ ψ : Formula α) : ~(φ ⋎ ψ) = (~φ) ⋏ (~ψ) := by rfl
 
+@[simp]
 def complexity : Formula α → ℕ
   | prime _ => 0
   | top => 0
@@ -67,45 +81,15 @@ def complexity : Formula α → ℕ
   | conj φ ψ => (max φ.complexity ψ.complexity) + 1
   | disj φ ψ => (max φ.complexity ψ.complexity) + 1
 
-/-
-lemma complexity0 {φ : Formula α} : φ.complexity = 0 → (φ.isPrime = true) := by
-  intro h;
-  cases φ with
-  | conj _ _ => simp [complexity] at h;
-  | disj _ _ => simp [complexity] at h;
-  | _ => rfl;
+attribute [simp] succ_le
 
-lemma complexity1 {φ : Formula α} : φ.complexity = 1 → (∃ (ψ ξ : Formula α), (ψ.isPrime = true ∧ ξ.isPrime = true) ∧ ((φ = ψ ⋏ ξ) ∨ (φ = ψ ⋎ ξ))) := by
-  intro h;
-  cases φ with
-  | conj ψ ξ => simp [complexity] at h; existsi ψ, ξ; exact ⟨⟨complexity0 h.left, complexity0 h.right⟩, Or.inl rfl⟩;
-  | disj ψ ξ => simp [complexity] at h; existsi ψ, ξ; exact ⟨⟨complexity0 h.left, complexity0 h.right⟩, Or.inr rfl⟩;
-  | _ => simp [complexity] at h;
--/
-/-
-def complexity₂ (φ : Formula α) : ℕ :=
-  if _ : isConnected φ then
-      match φ with
-      | conj φ ψ => (max φ.complexity ψ.complexity) + 1
-      | disj φ ψ => (max φ.complexity ψ.complexity) + 1
-    else 0
-
-@[simp] def complexity₂_atom {p : α} : complexity₂ (atom p) = 0 := rfl
-@[simp] def complexity₂_ctom {p : α} : complexity₂ (ctom p) = 0 := rfl
-@[simp] def complexity₂_top : complexity₂ (top : Formula α) = 0 := rfl
-@[simp] def complexity₂_bot : complexity₂ (bot : Formula α) = 0 := rfl
--/
-
-/-
-@[simp] lemma complexity_atom {p : α} : (atom p).complexity = 0 := rfl
-@[simp] lemma complexity_atom_upper {p : α} : (atom p).complexity < 1 := by simp [complexity]
--/
-
-@[simp] lemma complexity_conj2 {φ ψ : Formula α} : (max φ.complexity ψ.complexity) < ((φ ⋏ ψ).complexity) := by simp [complexity];
-@[simp] lemma complexity_disj2 {φ ψ : Formula α} : (max φ.complexity ψ.complexity) < ((φ ⋎ ψ).complexity) := by simp [complexity];
-
-@[simp] lemma complexity_conj_max {c} {φ ψ : Formula α} : ((φ ⋏ ψ).complexity ≤ c) → (φ.complexity < c ∧ ψ.complexity < c) := λ h => max_lt_iff.mp h
-@[simp] lemma complexity_disj_max {c} {φ ψ : Formula α} : ((φ ⋎ ψ).complexity ≤ c) → (φ.complexity < c ∧ ψ.complexity < c) := λ h => max_lt_iff.mp h
+@[simp] lemma complexity_prime : ((prime p).complexity < c + 1) := by aesop
+@[simp] lemma complexity_top : ((top : Formula α).complexity < c + 1) := by aesop
+@[simp] lemma complexity_bot : ((bot : Formula α).complexity < c + 1) := by aesop
+@[simp] lemma complexity_conj_le_lt_right {φ ψ : Formula α} : ((φ ⋏ ψ).complexity ≤ c) → (φ.complexity < c) := by aesop
+@[simp] lemma complexity_conj_le_lt_left {φ ψ : Formula α} : ((φ ⋏ ψ).complexity ≤ c) → (ψ.complexity < c) := by aesop
+@[simp] lemma complexity_disj_le_lt_right {φ ψ : Formula α} : ((φ ⋎ ψ).complexity ≤ c) → (φ.complexity < c) := by aesop;
+@[simp] lemma complexity_disj_le_lt_left {φ ψ : Formula α} : ((φ ⋎ ψ).complexity ≤ c) → (ψ.complexity < c) := by aesop
 
 end Formula
 
@@ -117,263 +101,235 @@ section Derivation
 
 variable {α : Type u} [DecidableEq α]
 
-inductive DerivationCR (CC : Formula α → Prop) : Sequent α → Type u where
-  | axm : ∀ (Γ) (p : α), ↑(+p) ∈ Γ → ↑(-p) ∈ Γ → DerivationCR CC Γ
-  | top : ∀ (Γ), Formula.top ∈ Γ → DerivationCR CC Γ
-  | conj : ∀ (Γ φ ψ), DerivationCR CC (insert φ $ Γ) → DerivationCR CC (insert ψ $ Γ) → DerivationCR CC (insert (φ ⋏ ψ) Γ)
-  | disj : ∀ (Γ φ ψ), DerivationCR CC (insert φ $ insert ψ $ Γ) → DerivationCR CC (insert (φ ⋎ ψ) Γ)
-  | cut : ∀ (Γ Δ φ), CC φ → DerivationCR CC (insert φ $ Γ) → DerivationCR CC (insert (~φ) $ Δ) → DerivationCR CC (Γ ∪ Δ)
-notation "⊢ᶜ[" CC "] " Γ => DerivationCR CC Γ
+inductive Derivation : ℕ → ℕ → Sequent α → Type u where
+  | Init : ∀ (Γ) (p : α), ↑(+p) ∈ Γ → ↑(-p) ∈ Γ → (∀ k c, Derivation k c Γ)
+  | Top : ∀ (Γ), Formula.top ∈ Γ → (∀ k c, Derivation k c Γ)
+  | Conj : ∀ {k c} {Γ φ ψ}, Derivation k c (insert φ $ Γ) → Derivation k c (insert ψ $ Γ) → (∀ {l d}, k < l → c ≤ d → Derivation l d (insert (φ ⋏ ψ) Γ))
+  | Disj : ∀ {k c} {Γ φ ψ}, Derivation k c (insert ψ $ insert φ $ Γ) → (∀ {l d}, k < l → c ≤ d → Derivation l d (insert (φ ⋎ ψ) Γ))
+  | Cut : ∀ {k c Γ Δ} (φ), (φ.complexity < c) → Derivation k c (insert φ $ Γ) → Derivation k c (insert (~φ) $ Δ) → (∀ {l d}, k < l → c ≤ d → Derivation l d (Γ ∪ Δ))
 
-abbrev DerivationWithoutCut (Γ : Sequent α) := ⊢ᶜ[λ _ => False] Γ
-notation "⊢ " Γ => DerivationWithoutCut Γ
+notation "⊢^{" k "}_{" c "} " Γ => Derivation k c Γ
 
-abbrev DerivationWithCut (Γ : Sequent α) :=  ⊢ᶜ[λ _ => True] Γ
-notation "⊢ᶜ " Γ => DerivationWithCut Γ
-
-abbrev DerivationLtCutComplexity (c : ℕ) (Γ : Sequent α) := ⊢ᶜ[λ φ => φ.complexity < c] Γ
-notation "⊢ᶜ[<" c "] " Γ => DerivationLtCutComplexity c Γ
-
-namespace DerivationCR
+namespace Derivation
 
 variable {α : Type u} [DecidableEq α]
 variable {Γ Δ : Sequent α}
 
-@[simp]
-def height {Γ : Sequent α} : DerivationCR P Γ → ℕ
-  | axm _ _ _ _ => 0
-  | top _ _ => 0
-  | conj _ _ _ D₁ D₂ => (max D₁.height D₂.height) + 1
-  | disj _ _ _ d => d.height + 1
-  | cut _ _ _ _ D₁ D₂ => (max D₁.height D₂.height) + 1
+@[simp] def cast {Γ : Sequent α} (he : Γ = Δ) : (⊢^{k}_{c} Γ) → (⊢^{k}_{c} Δ) := by subst he; exact λ d => d;
 
-@[simp]
-def height2 {Γ : Sequent α} : (⊢ᶜ[P] Γ) → (ℕ × ⊢ᶜ[P] Γ)
-  | axm Γ p ha hc => ⟨0, axm Γ p ha hc⟩
-  | top Γ ht => ⟨0, top Γ ht⟩
-  | conj Γ φ ψ D₁ D₂ => ⟨(max D₁.height D₂.height) + 1, conj Γ φ ψ D₁ D₂⟩
-  | disj Γ φ ψ D => ⟨D.height + 1, disj Γ φ ψ D⟩
-  | cut Γ₁ Γ₂ φ hp D₁ D₂ => ⟨(max D₁.height D₂.height) + 1, cut Γ₁ Γ₂ φ hp D₁ D₂⟩
+lemma liftHeight {Γ : Sequent α} (hh : k ≤ l) : (⊢^{k}_{c} Γ) → (⊢^{l}_{c} Γ)
+  | Init Γ p hatom hctom _ _ => Init Γ p hatom hctom l c
+  | Top Γ htop _ _ => Top Γ htop l c
+  | Conj Dφ Dψ hl hd => Conj Dφ Dψ (LT.lt.trans_le hl hh) hd
+  | Disj D hl hd => Disj D (LT.lt.trans_le hl hh) hd
+  | Cut _ hc Dl Dr hl hd => Cut _ hc Dl Dr (LT.lt.trans_le hl hh) hd
 
-/-
-@[simp] lemma height_axm (Γ : Sequent α) (p : α) (ha : atom p ∈ Γ) (hc : ctom p ∈ Γ) : (axm (P := P) Γ p ha hc).height = 0 := rfl
-@[simp] lemma height_top (Γ : Sequent α) (ht : Formula.top ∈ Γ) : (top (P := P) Γ ht).height = 0 := rfl
-@[simp] lemma height_conj (D₁ : ⊢ᶜ[P] (insert φ Γ)) (D₂ : ⊢ᶜ[P] (insert ψ Γ)) : (conj Γ φ ψ D₁ D₂).height = (max D₁.height D₂.height) + 1 := rfl
-@[simp] lemma height_disj (D : ⊢ᶜ[P] (insert φ $ insert ψ Γ)) : (disj Γ φ ψ D).height = D.height + 1 := rfl
-@[simp] lemma height_cut (D₁ : ⊢ᶜ[P] (insert φ Γ)) (D₂ : ⊢ᶜ[P] (insert (~φ) Δ)) : (cut Γ Δ φ hp D₁ D₂).height = (max D₁.height D₂.height) + 1 := rfl
--/
+lemma weakening {Γ : Sequent α} (hk : k ≤ k') (hc : c ≤ c') (hΓ : Γ ⊆ Γ') : (⊢^{k}_{c} Γ) → (⊢^{k'}_{c'} Γ')
+  | Init Γ p hatom hctom _ _ => Init Γ' p (hΓ hatom) (hΓ hctom) k' c'
+  | Top Γ htop _ _ => Top Γ' (hΓ htop) k' c'
+  | @Conj _ _ l d Γ φ ψ Dφ Dψ _ _ hl hd => by
+      have wD₁ : ⊢^{l}_{d} insert φ Γ' := Dφ.weakening (by simp) (by simp) (insert_subset_insert φ (insert_subset_iff.mp hΓ).2);
+      have wD₂ : ⊢^{l}_{d} insert ψ Γ' := Dψ.weakening (by simp) (by simp) (insert_subset_insert ψ (insert_subset_iff.mp hΓ).2);
+      exact (Conj wD₁ wD₂ (LT.lt.trans_le hl hk) (LE.le.trans hd hc)).cast (by simp [insert_eq_self]; apply hΓ; simp;);
+  | @Disj _ _ l d Γ φ ψ D _ _ hl hd => by
+      have wD : ⊢^{l}_{d} insert ψ $ insert φ Γ' := D.weakening (by simp) (by simp) (insert_subset_insert ψ $ insert_subset_insert φ $ (insert_subset_iff.mp hΓ).2);
+      exact (Disj wD (LT.lt.trans_le hl hk) (LE.le.trans hd hc)).cast (by simp [insert_eq_self]; apply hΓ; simp;);
+  | @Cut _ _ l d Γ Δ φ hcomplex Dl Dr _ _ hl hd => by
+      have wDl : ⊢^{l}_{d} insert φ Γ' := Dl.weakening (by simp) (by simp) (insert_subset_insert _ (union_subset_left hΓ));
+      have wDr : ⊢^{l}_{d} (insert (~φ) Γ') := Dr.weakening (by simp) (by simp) (insert_subset_insert _ (union_subset_right hΓ));
+      exact (Cut _ hcomplex wDl wDr (LT.lt.trans_le hl hk) (LE.le.trans hd hc)).cast (by simp);
 
-@[simp] def cast (he : Γ = Δ) : (⊢ᶜ[P] Γ) → (⊢ᶜ[P] Δ) := by subst he; exact λ d => d;
-@[simp] lemma cast_HeightPreserving (h : ⊢ᶜ[P] Γ) (he : Γ = Δ) : (h.cast he).height = h.height := by subst he; trivial;
+lemma inversionDisjAux {Γ : Sequent α} : (⊢^{k}_{c} Γ) → (∀ φ ψ, ⊢^{k}_{c} insert ψ $ insert φ $ Γ.erase (φ ⋎ ψ))
+  | Init Γ p hatom hctom _ _, φ, ψ => Init _ p (by simp [hatom]) (by simp [hctom]) k c
+  | Top Γ htop _ _, φ, ψ => Top _ (by simp [htop]) k c
+  | @Conj _ _ l d Γ ξ ζ Dξ Dζ _ _ hl hd, φ, ψ => by
+      have hD₁ : ⊢^{l}_{d} insert ξ $ insert ψ $ insert φ $ erase Γ (φ ⋎ ψ) := (Dξ.inversionDisjAux φ ψ).weakening (by simp) (by simp)
+          (by simp [subset_iff]; rintro x hx (rfl | hhx) <;> simp [*]);
+      have hD₂ : ⊢^{l}_{d} insert ζ $ insert ψ $ insert φ $ erase Γ (φ ⋎ ψ) := (Dζ.inversionDisjAux φ ψ).weakening (by simp) (by simp)
+          (by simp [subset_iff]; rintro x hx (rfl | hhx) <;> simp [*]);
+      exact (Conj hD₁ hD₂ hl hd).cast (by simp [erase_insert_of_ne, Finset.Insert.comm]);
+  | @Disj _ _ l d Γ φ ψ D _ _ hl hd, ξ, ζ => by
+      by_cases e : (φ = ξ) ∧ (ψ = ζ);
+      . exact @weakening _ _ (l + 1) k d c _ _ (by aesop) hd (by simp [subset_iff, e]; rintro χ hχ (rfl | hhx) <;> simp [*]) ((D.inversionDisjAux φ ψ).liftHeight (by simp));
+      . have ne : (φ ⋎ ψ) ≠ (ξ ⋎ ζ) := disj_neq (not_and_or.mp e);
+        have hD : ⊢^{l}_{d} insert ψ $ insert φ $ insert ζ $ insert ξ $ erase Γ (ξ ⋎ ζ) := (D.inversionDisjAux ξ ζ).weakening (by simp) (by simp)
+          (by simp [subset_iff]; rintro x hx (rfl | rfl | hhx) <;> simp [*]);
+        exact (Disj hD hl hd).cast (by simp [erase_insert_of_ne ne, Finset.Insert.comm]);
+  | @Cut _ _ l d Γ Δ φ hcomplex Dl Dr _ _ hl hd, ξ, ζ => by
+      have hDl : ⊢^{l}_{d} insert φ $ insert ζ $ insert ξ (erase Γ (ξ ⋎ ζ)) := (Dl.inversionDisjAux ξ ζ).weakening (by simp) (by simp)
+        (by simp [subset_iff]; rintro x hx (rfl | hhx) <;> simp [*]);
+      have hDr : ⊢^{l}_{d} insert (~φ) $ insert ζ $ insert ξ (erase Δ (ξ ⋎ ζ)) := (Dr.inversionDisjAux ξ ζ).weakening (by simp) (by simp)
+        (by simp [subset_iff]; rintro x hx (rfl | hhx) <;> simp [*]);
+      exact (Cut _ hcomplex hDl hDr hl hd).cast (by simp [erase_union];);
 
-def replaceCondition {Γ : Sequent α} {P Q : Formula α → Prop} (h : ∀ φ, P φ → Q φ) : (⊢ᶜ[P] Γ) → (⊢ᶜ[Q] Γ)
-  | axm Γ p ha hc => axm Γ p ha hc
-  | top Γ ht => top Γ ht
-  | conj Γ φ ψ D₁ D₂ => conj Γ φ ψ (D₁.replaceCondition h) (D₂.replaceCondition h)
-  | disj Γ φ ψ D => disj Γ φ ψ (D.replaceCondition h)
-  | cut Γ₁ Γ₂ φ hp D₁ D₂ => cut Γ₁ Γ₂ φ (h φ hp) (D₁.replaceCondition h) (D₂.replaceCondition h)
+lemma inversionDisj {Γ : Sequent α} (D : (⊢^{k}_{c} insert (φ ⋎ ψ) Γ)) : (⊢^{k}_{c} insert ψ $ insert φ Γ) := by
+  apply (D.inversionDisjAux φ ψ).weakening <;> simp [insert_subset_insert, erase_subset];
 
-lemma liftCutComplexity (h : i ≤ j) : (⊢ᶜ[< i] Γ) → (⊢ᶜ[< j] Γ) := replaceCondition (λ _ hp => Nat.lt_of_lt_of_le hp h)
+lemma inversionConjLAux {Γ : Sequent α} : (⊢^{k}_{c} Γ) → (∀ φ ψ, ⊢^{k}_{c} insert φ $ Γ.erase (φ ⋏ ψ))
+  | Init Γ p hatom hctom _ _, φ, ψ => Init _ p (by simp [hatom]) (by simp [hctom]) k c
+  | Top Γ htop _ _, φ, ψ => Top _ (by simp [htop]) k c
+  | @Conj _ _ l d Γ ξ ζ Dξ Dζ _ _ hl hd, φ, ψ => by
+      by_cases e : (ξ = φ) ∧ (ζ = ψ);
+      . exact @weakening _ _ (l + 1) k d c _ _ (by aesop) hd (by simp [subset_iff]; rintro χ hχ (rfl | hhx) <;> simp [*]) ((Dξ.inversionConjLAux φ ψ).liftHeight (by simp));
+      . have ne : (ξ ⋏ ζ) ≠ (φ ⋏ ψ) := conj_neq (not_and_or.mp e);
+        have hD₁ : ⊢^{l}_{d} insert ξ $ insert φ $ erase Γ (φ ⋏ ψ) := (Dξ.inversionConjLAux φ ψ).weakening (by simp) (by simp)
+          (by simp [subset_iff]; rintro x hx (rfl | hhx) <;> simp [*]);
+        have hD₂ : ⊢^{l}_{d} insert ζ $ insert φ $ erase Γ (φ ⋏ ψ) := (Dζ.inversionConjLAux φ ψ).weakening (by simp) (by simp)
+          (by simp [subset_iff]; rintro x hx (rfl | hhx) <;> simp [*]);
+        exact (Conj hD₁ hD₂ hl hd).cast (by simp [erase_insert_of_ne ne, Insert.comm φ]);
+  | @Disj _ _ l d Γ ξ ζ D _ _ hl hd, φ, ψ => by
+      have hD : ⊢^{l}_{d} insert ζ $ insert ξ $ insert φ $ (erase Γ (φ ⋏ ψ)) := (D.inversionConjLAux φ ψ).weakening (by simp) (by simp)
+        (by simp [subset_iff]; rintro χ hχ (rfl | rfl | hhx) <;> simp [*]);
+      exact (Disj hD hl hd).cast (by simp [erase_insert_of_ne, Insert.comm φ])
+  | @Cut _ _ l d Γ Δ ξ hcomplex Dl Dr _ _ hl hd, φ, ψ => by
+      have hDl : ⊢^{l}_{d} insert ξ $ insert φ (erase Γ (φ ⋏ ψ)) := (Dl.inversionConjLAux φ ψ).weakening (by simp) (by simp)
+        (by simp [subset_iff]; rintro x hx (rfl | hhx) <;> simp [*]);
+      have hDr : ⊢^{l}_{d} insert (~ξ) $ insert φ (erase Δ (φ ⋏ ψ)) := (Dr.inversionConjLAux φ ψ).weakening (by simp) (by simp)
+        (by simp [subset_iff]; rintro x hx (rfl | hhx) <;> simp [*]);
+      exact (Cut _ hcomplex hDl hDr hl hd).cast (by simp [erase_union];);
 
-def weakening {Γ: Sequent α} : (⊢ᶜ[P] Γ) → (∀ {Δ : Sequent α}, Γ ⊆ Δ → ⊢ᶜ[P] Δ)
-  | axm Γ p ha hc, Δ, h => axm Δ p (h ha) (h hc)
-  | top Γ ht, Δ, h => top Δ (h ht)
-  | conj Γ φ ψ D₁ D₂, Δ, h =>
-      let wD₁ : ⊢ᶜ[P] insert φ Δ := D₁.weakening (insert_subset_insert φ (insert_subset_iff.mp h).2);
-      let wD₂ : ⊢ᶜ[P] insert ψ Δ := D₂.weakening (insert_subset_insert ψ (insert_subset_iff.mp h).2);
-      (conj Δ φ ψ wD₁ wD₂).cast (by simp; exact (insert_subset_iff.mp h).1)
-  | disj Γ φ ψ D, Δ, h =>
-      let wD : ⊢ᶜ[P] (insert φ $ insert ψ Δ) := D.weakening (insert_subset_insert φ (insert_subset_insert ψ (insert_subset_iff.mp h).2));
-      (disj Δ φ ψ wD).cast (by simp; exact (insert_subset_iff.mp h).1)
-  | cut Γ₁ Γ₂ φ hp D₁ D₂, Δ, h =>
-      let wD₁ : ⊢ᶜ[P] (insert φ Δ) := D₁.weakening (insert_subset_insert _ (union_subset_left h));
-      let wD₂ : ⊢ᶜ[P] (insert (~φ) Δ) := D₂.weakening (insert_subset_insert _ (union_subset_right h));
-      (cut Δ Δ φ hp wD₁ wD₂).cast (by simp)
+lemma inversionConjL {Γ : Sequent α} (D : (⊢^{k}_{c} insert (φ ⋏ ψ) Γ)) : (⊢^{k}_{c} insert φ Γ) := by
+  apply (D.inversionConjLAux φ ψ).weakening <;> simp [insert_subset_insert, erase_subset];
 
-def weakening₁ : (⊢ᶜ[P] Γ) → (∀ {φ}, ⊢ᶜ[P] (insert φ Γ)) := by
-  intro D φ;
-  exact D.weakening (subset_insert φ Γ)
+lemma inversionConjRAux {Γ : Sequent α} : (⊢^{k}_{c} Γ) → (∀ φ ψ, ⊢^{k}_{c} insert ψ $ Γ.erase (φ ⋏ ψ))
+  | Init Γ p hatom hctom _ _, φ, ψ => Init _ p (by simp [hatom]) (by simp [hctom]) k c
+  | Top Γ htop _ _, φ, ψ => Top _ (by simp [htop]) k c
+  | @Conj _ _ l d Γ ξ ζ Dξ Dζ _ _ hl hd, φ, ψ => by
+      by_cases e : (ξ = φ) ∧ (ζ = ψ);
+      . exact @weakening _ _ (l + 1) k d c _ _ (by aesop) hd (by simp [subset_iff]; rintro χ hχ (rfl | hhx) <;> simp [*]) ((Dζ.inversionConjRAux φ ψ).liftHeight (by simp));
+      . have ne : (ξ ⋏ ζ) ≠ (φ ⋏ ψ) := conj_neq (not_and_or.mp e);
+        have hD₁ : ⊢^{l}_{d} insert ξ $ insert ψ $ erase Γ (φ ⋏ ψ) := (Dξ.inversionConjRAux φ ψ).weakening (by simp) (by simp)
+          (by simp [subset_iff]; rintro x hx (rfl | hhx) <;> simp [*]);
+        have hD₂ : ⊢^{l}_{d} insert ζ $ insert ψ $ erase Γ (φ ⋏ ψ) := (Dζ.inversionConjRAux φ ψ).weakening (by simp) (by simp)
+          (by simp [subset_iff]; rintro x hx (rfl | hhx) <;> simp [*]);
+        exact (Conj hD₁ hD₂ hl hd).cast (by simp [erase_insert_of_ne ne, Insert.comm ψ]);
+  | @Disj _ _ l d Γ ξ ζ D _ _ hl hd, φ, ψ => by
+      have hD : ⊢^{l}_{d} insert ζ $ insert ξ $ insert ψ $ (erase Γ (φ ⋏ ψ)) := (D.inversionConjRAux φ ψ).weakening (by simp) (by simp)
+        (by simp [subset_iff]; rintro χ hχ (rfl | rfl | hhx) <;> simp [*]);
+      exact (Disj hD hl hd).cast (by simp[Finset.erase_insert_of_ne, Finset.Insert.comm ψ])
+  | @Cut _ _ l d Γ Δ ξ hcomplex Dl Dr _ _ hl hd, φ, ψ => by
+      have hDl : ⊢^{l}_{d} insert ξ $ insert ψ (erase Γ (φ ⋏ ψ)) := (Dl.inversionConjRAux φ ψ).weakening (by simp) (by simp)
+        (by simp [subset_iff]; rintro x hx (rfl | hhx) <;> simp [*]);
+      have hDr : ⊢^{l}_{d} insert (~ξ) $ insert ψ (erase Δ (φ ⋏ ψ)) := (Dr.inversionConjRAux φ ψ).weakening (by simp) (by simp)
+        (by simp [subset_iff]; rintro x hx (rfl | hhx) <;> simp [*]);
+      exact (Cut _ hcomplex hDl hDr hl hd).cast (by simp [erase_union];);
 
-lemma weakening_HeightPreserving (D : ⊢ᶜ[P] Γ) (h : Γ ⊆ Δ) : (D.weakening h).height = D.height := by
-  induction D generalizing Δ <;> simp [weakening, height];
-  sorry;
-  sorry;
-  sorry;
+lemma inversionConjR {Γ : Sequent α} (D : (⊢^{k}_{c} insert (φ ⋏ ψ) Γ)) : (⊢^{k}_{c} insert ψ Γ) := by
+  apply (D.inversionConjRAux φ ψ).weakening <;> simp [insert_subset_insert, erase_subset];
 
-def inversionDisjAux {Γ : Sequent α} : (⊢ᶜ[CC] Γ) → (∀ φ ψ, ⊢ᶜ[CC] insert ψ $ insert φ $ Γ.erase (φ ⋎ ψ))
-  | axm Γ p ha hc, φ, ψ => axm _ p (by simp [ha]) (by simp [hc])
-  | top Γ ht, φ, ψ => top _ (by simp [ht])
-  | conj Γ φ ψ D₁ D₂, φ', ψ' =>
-      have iD₁ := D₁.inversionDisjAux φ' ψ';
-      have iD₂ := D₂.inversionDisjAux φ' ψ';
-      sorry
-      -- let iD₁ := D₁.inversionDisj φ' ψ';
-      -- let iD₂ := D₂.inversionDisj φ' ψ';
-      -- (conj _ _ _ iD₁ iD₂).cast (by sorry)
-  | disj Γ φ ψ D, φ', ψ' => sorry
-      -- let iD : ⊢ᶜ[P] (insert φ $ insert ψ $ Γ.erase (φ' ⋎ ψ')) := D.inversionDisj φ' ψ';
-      -- (disj _ _ _ iD).cast (by simp)
-  | cut Γ₁ Γ₂ φ hp D₁ D₂, φ', ψ' => sorry
-      -- let iD₁ : ⊢ᶜ[P] (insert φ $ Γ₁.erase (φ' ⋎ ψ')) := D₁.inversionDisj φ' ψ';
-      -- let iD₂ : ⊢ᶜ[P] (insert (~φ) $ Γ₂.erase (φ' ⋎ ψ')) := D₂.inversionDisj φ' ψ';
-      -- (cut _ _ _ hp iD₁ iD₂).cast (by simp)
+lemma reduction {Γ Δ : Sequent α} {φ : Formula α} (hc : φ.complexity ≤ c + 1) : (⊢^{k}_{c + 1} (insert φ Γ)) → (⊢^{k}_{c + 1} (insert (~φ) Δ)) → (⊢^{k + 2}_{c + 1} (Γ ∪ Δ)) := by
+  intro Dl Dr;
+  cases φ with
+  | conj φ ψ =>
+      have C₁ : ⊢^{k + 1}_{c + 1} (insert (neg φ) (Γ ∪ Δ)) := (Cut _ (complexity_conj_le_lt_left hc) Dl.inversionConjR Dr.inversionDisj (by simp) (by simp)).cast (by simp);
+      have C₂ : ⊢^{k + 2}_{c + 1} (Γ ∪ Δ) := (Cut _ (complexity_conj_le_lt_right hc) (Dl.inversionConjL.liftHeight (by simp)) C₁ (by simp) (by simp)).cast (by simp);
+      exact C₂;
+  | disj φ ψ =>
+      have C₁ : ⊢^{k + 1}_{c + 1} (insert φ (Γ ∪ Δ)) := (Cut _ (complexity_disj_le_lt_left hc) Dl.inversionDisj Dr.inversionConjR (by simp) (by simp)).cast (by simp);
+      have C₂ : ⊢^{k + 2}_{c + 1} (Γ ∪ Δ) := (Cut _ (complexity_disj_le_lt_right hc) C₁ (Dr.inversionConjL.liftHeight (by simp)) (by simp) (by simp)).cast (by simp);
+      exact C₂;
+  | _ => exact Cut _ (by simp) Dl Dr (by simp) (by simp);
 
-def inversionDisj {Γ : Sequent α} (D : (⊢ᶜ[P] insert (φ ⋎ ψ) Γ)) : (⊢ᶜ[P] insert ψ $ insert φ Γ) := by
-  apply (D.inversionDisjAux φ ψ).weakening;
-  apply insert_subset_insert;
-  apply insert_subset_insert;
-  apply erase_insert_subset;
+lemma reductionPrime {Γ Δ : Sequent α} {p : α} : (⊢^{k}_{0} (insert ↑(+p) Γ)) → (⊢^{l}_{0} (insert ↑(-p) Δ)) → (⊢^{k + l}_{0} (Γ ∪ Δ)) := by
+  intro D₁ D₂;
+  induction k with
+  | zero =>
+    cases D₁ with
+    | Init Γ q hatom hctom =>
+        by_cases hpq : p = q
+        . simp_all [hpq];
+        . apply Init _ q (by aesop) (by aesop);
+    | Top Γ htop => apply Top (Γ ∪ Δ) (by aesop);
+      -- have C₂ : ⊢^{l}_{0} (insert (↑p) (Γ ∪ Δ)) := (Cut _ (by simp) D₁ C₁ (by simp) (by simp)).cast (by simp);
+  | succ k ih =>
+      sorry;
 
-def inversionConjLAux {Γ : Sequent α} : (⊢ᶜ[P] Γ) → (∀ φ ψ, ⊢ᶜ[P] insert φ $ Γ.erase (φ ⋏ ψ))
-  | axm Γ p ha hc, φ, ψ => axm _ p (by simp [ha]) (by simp [hc])
-  | top Γ ht, φ, ψ => top _ (by simp [ht])
-  | conj Γ φ' ψ' Dφ Dψ, φ, ψ => by
-      by_cases e : (φ' = φ) ∧ (ψ' = ψ)
-      . exact (inversionConjLAux Dφ φ ψ).weakening (by simp [subset_iff]; intro ξ hξ; sorry;)
-      . have n : (φ ⋏ ψ) ≠ (φ' ⋏ ψ') := by sorry;
-
-        have Dφ' : ⊢ᶜ[P] (insert φ' $ insert φ $ Γ.erase (φ' ⋏ ψ')) := sorry;
-        have Dψ' : ⊢ᶜ[P] (insert ψ' $ insert φ $ Γ.erase (φ' ⋏ ψ')) := sorry;
-        apply (conj _ _ _ Dφ' Dψ').cast;
-        sorry;
-        -- simp [erase_insert_of_ne];
-
-        -- have Dφ : ⊢ᶜ[P] insert φ $ Γ.erase (φ' ⋏ ψ') := D₁.inversionConj φ' ψ';
-  | disj Γ φ ψ D, ξ, χ => by
-      have DΓ := D.inversionConjLAux ξ χ;
-      sorry
-      -- apply (disj _ _ _ DΓ).cast;
-
-  | cut Γ₁ Γ₂ φ hp D₁ D₂, ψ, ξ => by
-      have DΓ₁ : ⊢ᶜ[P] insert φ $ insert ψ (erase Γ₁ (ψ ⋏ ξ)) := (D₁.inversionConjLAux ψ ξ).weakening (by simp [subset_iff]; intro ζ hζ; sorry;);
-      have DΓ₂ : ⊢ᶜ[P] insert (~φ) $ insert ψ (erase Γ₂ (ψ ⋏ ξ)) := (D₂.inversionConjLAux ψ ξ).weakening (by simp [subset_iff]; intro ζ hζ; sorry;);
-      apply (cut _ _ _ hp DΓ₁ DΓ₂).cast;
-      simp [erase_union];
-
-  /--
-  | disj Γ φ ψ D, φ', ψ' =>
-      let iD : ⊢ᶜ[P] (insert φ $ insert ψ $ Γ.erase (φ' ⋎ ψ')) := D.inversionDisj φ' ψ';
-      (disj _ _ _ iD).cast (by simp)
-  | cut Γ₁ Γ₂ φ hp D₁ D₂, φ', ψ' =>
-      let iD₁ : ⊢ᶜ[P] (insert φ $ Γ₁.erase (φ' ⋎ ψ')) := D₁.inversionDisj φ' ψ';
-      let iD₂ : ⊢ᶜ[P] (insert (~φ) $ Γ₂.erase (φ' ⋎ ψ')) := D₂.inversionDisj φ' ψ';
-      (cut _ _ _ hp iD₁ iD₂).cast (by simp)
--/
-
-def inversionConjL {Γ : Sequent α} (D : (⊢ᶜ[P] insert (φ ⋏ ψ) Γ)) : (⊢ᶜ[P] insert φ Γ) := by
-  apply (D.inversionConjLAux φ ψ).weakening;
-  apply insert_subset_insert;
-  apply erase_insert_subset;
-
-def inversionConjRAux {Γ : Sequent α} : (⊢ᶜ[P] Γ) → (∀ φ ψ, ⊢ᶜ[P] insert ψ $ Γ.erase (φ ⋏ ψ))
-  | axm Γ p ha hc, φ, ψ => axm _ p (by simp [ha]) (by simp [hc])
-  | top Γ ht, φ, ψ => top _ (by simp [ht])
-  | conj Γ φ' ψ' Dφ Dψ, φ, ψ => by
-      by_cases e : (φ' = φ) ∧ (ψ' = ψ)
-      . exact (inversionConjRAux Dφ φ ψ).weakening (by simp [subset_iff]; intro ξ hξ; sorry;)
-      . have n : (φ ⋏ ψ) ≠ (φ' ⋏ ψ') := by sorry;
-        have Dφ' : ⊢ᶜ[P] (insert φ' $ insert φ $ Γ.erase (φ' ⋏ ψ')) := sorry;
-        have Dψ' : ⊢ᶜ[P] (insert ψ' $ insert φ $ Γ.erase (φ' ⋏ ψ')) := sorry;
-        apply (conj _ _ _ Dφ' Dψ').cast;
-        sorry
-  | disj Γ φ ψ D, φ', ψ' => sorry
-  | cut Γ₁ Γ₂ φ hp D₁ D₂, φ', ψ' => sorry
-
-def inversionConjR {Γ : Sequent α} (D : (⊢ᶜ[P] insert (φ ⋏ ψ) Γ)) : (⊢ᶜ[P] insert ψ Γ) := by
-  apply (D.inversionConjRAux φ ψ).weakening;
-  apply insert_subset_insert;
-  apply erase_insert_subset;
-
-lemma inversionDisj_HeightPreserving (D : ⊢ᶜ[P] Γ) : (D.inversionDisjAux φ ψ).height = D.height := by
-  induction D <;>
-  simp [inversionDisj, height];
-  sorry;
-  sorry;
-  sorry;
-
-lemma inversionConjL_HeightPreserving (D : ⊢ᶜ[P] Γ) : (D.inversionConjLAux φ ψ).height = D.height := by
-  induction D <;>
-  simp [inversionConjL, height];
-  sorry;
-  sorry;
-  sorry;
-
-lemma inversionConjR_HeightPreserving (D : ⊢ᶜ[P] Γ) : (D.inversionConjRAux φ ψ).height = D.height := by
-  induction D <;>
-  simp [inversionConjR, height];
-  sorry;
-  sorry;
-  sorry;
-
-lemma reduceCut1 {Γ : Sequent α} : (⊢ᶜ[< 1] Γ) → (⊢ᶜ[< 0] Γ)
-  | axm Γ p ha hc => axm Γ p ha hc
-  | top Γ ht => top Γ ht
-  | conj Γ φ ψ Dφ Dψ => conj _ _ _ (Dφ.reduceCut1) (Dψ.reduceCut1)
-  | disj Γ φ ψ D => disj Γ φ ψ (D.reduceCut1)
-  | cut _ _ φ hcut D₁ D₂ =>
+lemma reduceCut1 {Γ : Sequent α} : (⊢^{k}_{1} Γ) → (⊢^{k}_{0} Γ)
+  | Init Γ p hatom hctom _ _ => Init Γ p hatom hctom k 0
+  | Top Γ htop _ _ => Top Γ htop k 0
+  | Conj Γ φ ψ Dφ Dψ => Conj _ _ _ (Dφ.reduceCut1) (Dψ.reduceCut1)
+  | Disj Γ φ ψ D => Disj Γ φ ψ (D.reduceCut1)
+  | Cut Γ₁ Γ₂ φ hCut D₁ D₂ =>
     match φ with
     | .prime p => by sorry; -- reductionPrime (red D₁) (red D₂)
     | .top => by sorry;
     | .bot => by sorry;
 
-lemma reduction {Γ Δ : Sequent α} {φ : Formula α} (hc : φ.complexity ≤ c + 1) : (⊢ᶜ[< c + 1] (insert φ Γ)) → (⊢ᶜ[< c + 1] (insert (~φ) Δ)) → (⊢ᶜ[< c + 1] (Γ ∪ Δ)) := by
-  intro D₁ D₂;
-  cases φ with
-  | conj φ ψ =>
-    have C₁ : ⊢ᶜ[< c + 1] insert (~φ) (Γ ∪ Δ) := by have := cut _ _ _ ((complexity_conj_max hc).2) (inversionConjR D₁) (inversionDisj D₂); simp [insert_union] at this; exact this;
-    have C₂ : ⊢ᶜ[< c + 1] Γ ∪ Δ := by have := cut _ _ _ ((complexity_conj_max hc).1) (inversionConjL D₁) C₁; simp [insert_union] at this; exact this;
-    exact C₂;
-  | disj φ ψ =>
-    have C₁ : ⊢ᶜ[< c + 1] insert φ (Γ ∪ Δ) := by have := cut _ _ _ ((complexity_disj_max hc).2) D₁.inversionDisj D₂.inversionConjR; simp [insert_union] at this; exact this;
-    have C₂ : ⊢ᶜ[< c + 1] Γ ∪ Δ := by have := cut _ _ _ ((complexity_disj_max hc).1) C₁ D₂.inversionConjL; simp at this; exact this;
-    exact C₂;
-  | _ => exact cut _ _ _ (by simp [complexity]) D₁ D₂;
+lemma reduceCutLt2 {Γ : Sequent α} : (⊢^{k}_{c + 1} Γ) → (⊢^{2 ^ k}_{c} Γ)
+  | Init Γ p hatom hctom _ _ => by apply Init _ _ hatom hctom;
+  | Top Γ htop _ _ => by apply Top _ htop;
+  | Conj Dφ Dψ _ _ => reduceCutLt2 $ Conj Dφ Dψ (by assumption) (by assumption)
+  | Disj D _ _ => reduceCutLt2 $ Disj D (by assumption) (by assumption)
+  | @Cut _ _ l d Γl Γr  φ hcomplex Dl Dr _ _ hl hd =>
+      -- have RR := Dr.reduceCutLt2;
+      -- have := reduction (by sorry) (Dl.reduceCutLt2) (Dr.reduceCutLt2);
+      -- match φ with
+      -- | .prime p => sorry -- reductionPrime (Dl.reduceCutLt2) (Dr.reduceCutLt2)
+      -- | .top => sorry
+      -- | .bot => sorry
+      -- | .conj φ ψ => sorry -- reduction (Nat.lt_add_one_iff.mp hcomplex) (Dl.reduceCutLt2) (Dr.reduceCutLt2)
+      -- | .disj φ ψ => sorry
+-- termination_by reduceCutLt2 D => by sorry
+      -- have hDl := reduceCutLt2;
+      -- have hDr := @reduceCutLt2 k c (insert φ Γr);
+      -- sorry;
 
-lemma reductionPrime {Γ Δ : Sequent α} {p : Prime α} : (⊢ᶜ[< c] (insert ↑p Γ)) → (⊢ᶜ[< c] (insert (~↑p) Δ)) → (⊢ᶜ[< c] (Γ ∪ Δ)) := by
-  intro D₁ D₂;
-  cases p with
-  | _ p =>
-    let k := D₁.height;
-    induction k with
-    | zero => sorry;
-    | succ n ih => sorry; -- exact ih;
-  -- | conj => simp [isPrime] at hp;
-  -- | disj => simp [isPrime] at hp;
-  -- | _ => exact cut _ _ _ (by simp [complexity]; exact hc) D₁ D₂;
+      -- induction c with
+      -- | zero =>
+      --     have hDl : ⊢^{k}_{0} (insert φ Δl) := Dl.reduceCut1;
+      --     have hDr : ⊢^{k}_{0} (insert (~φ) Δr) := Dr.reduceCut1;
+      --     exact (Cut hcomplex hDl hDr hk hc).cast (by simp);
+      -- | succ c ih =>
+      --     have hDl := Dl.reduceCutLt2;
+      --     have hDr := Dr.reduceCutLt2;
 
+          -- exact (Cut hcomplex hDl hDr hk hc).cast (by simp);
+
+  -- | @Cut _ _ l d Δl Δr φ hcomplex Dl Dr _ _ hl hd => by
+    /-
+      match φ with
+      | .prime p => by sorry; -- reductionPrime (red Dl) (red Dr)
+      | .top => by sorry;
+      | .bot => by sorry;
+      | .conj φ ψ => by sorry;
+      | .disj φ ψ => have a := (D₁.reduceCutLt2); have b := (D₂.reduceCutLt2);
+-/
+/-
 noncomputable def reduceCutLt2 {Γ : Sequent α} : (⊢ᶜ[< c + 2] Γ) → (⊢ᶜ[< c + 1] Γ)
-  | axm Γ p ha hc => axm Γ p ha hc
+  | Init Γ p ha hc => Init Γ p ha hc
   | top Γ ht => top Γ ht
   | conj Γ φ ψ Dφ Dψ => conj Γ φ ψ (Dφ.reduceCutLt2) (Dψ.reduceCutLt2)
   | disj Γ φ ψ D => disj Γ φ ψ (D.reduceCutLt2)
-  | cut _ _ φ hcut D₁ D₂ =>
+  | Cut _ _ φ hCut D₁ D₂ =>
     match φ with
     | .prime _ => reductionPrime (D₁.reduceCutLt2) (D₂.reduceCutLt2)
-    | _ => reduction (Nat.lt_add_one_iff.mp hcut) (D₁.reduceCutLt2) (D₂.reduceCutLt2)
+    | _ => reduction (Nat.lt_add_one_iff.mp hCut) (D₁.reduceCutLt2) (D₂.reduceCutLt2)
+-/
 
-noncomputable def CutElimination' {Γ : Sequent α} : {c : ℕ} → (⊢ᶜ[< c] Γ) → (⊢ Γ)
-  | 0, D => D.replaceCondition (by simp)
-  | 1, D => D.reduceCut1.CutElimination'
-  | _ + 2, D => (D.reduceCutLt2).CutElimination'
+lemma CutElimination {Γ : Sequent α} : {c : ℕ} → (⊢^{k}_{c} Γ) → (⊢^{2 ^ (2 ^ k * m)}_{0} Γ)
+  | 0, D => sorry -- D.replaceCondition (by simp)
+  | c + 1, D => sorry
 
-noncomputable def cutMax {Γ : Sequent α} : (⊢ᶜ Γ) → ((c : ℕ) × (⊢ᶜ[< c] Γ))
-  | axm Γ p ha hc => ⟨0, axm Γ p ha hc⟩
+/-
+noncomputable def CutMax {Γ : Sequent α} : (⊢^{k}_{c} Γ) → ((c : ℕ) × (⊢ᶜ[< c] Γ))
+  | Init Γ p ha hc => ⟨0, Init Γ p ha hc⟩
   | top Γ ht => ⟨0, top Γ ht⟩
   | conj Γ φ ψ Dφ Dψ =>
-      let ⟨c₁, D₁⟩ := Dφ.cutMax;
-      let ⟨c₂, D₂⟩ := Dψ.cutMax;
+      let ⟨c₁, D₁⟩ := Dφ.CutMax;
+      let ⟨c₂, D₂⟩ := Dψ.CutMax;
       ⟨max c₁ c₂, conj Γ φ ψ (D₁.liftCutComplexity (by simp)) (D₂.liftCutComplexity (by simp))⟩
   | disj Γ φ ψ D =>
-      let ⟨c, D⟩ := D.cutMax;
+      let ⟨c, D⟩ := D.CutMax;
       ⟨c, disj Γ φ ψ (D.liftCutComplexity (by simp))⟩
-  | cut Γ₁ Γ₂ φ _ D₁ D₂ =>
-      let ⟨c₁, D₁⟩ := D₁.cutMax;
-      let ⟨c₂, D₂⟩ := D₂.cutMax;
-      ⟨max (max c₁ c₂) (φ.complexity + 1), cut Γ₁ Γ₂ φ (by simp) (D₁.liftCutComplexity (by simp)) (D₂.liftCutComplexity (by simp))⟩
+  | Cut Γ₁ Γ₂ φ _ D₁ D₂ =>
+      let ⟨c₁, D₁⟩ := D₁.CutMax;
+      let ⟨c₂, D₂⟩ := D₂.CutMax;
+      ⟨max (max c₁ c₂) (φ.complexity + 1), Cut Γ₁ Γ₂ φ (by simp) (D₁.liftCutComplexity (by simp)) (D₂.liftCutComplexity (by simp))⟩
 
-noncomputable def cutElimination : (⊢ᶜ Γ) → (⊢ Γ) := λ D => (D.cutMax.2).CutElimination'
+noncomputable def CutElimination : (⊢ᶜ Γ) → (⊢ Γ) := λ D => (D.CutMax.2).CutElimination'
+-/
 
-end DerivationCR
+end Derivation
 
 end Derivation
 
